Plfl/Untyped/Denotational/Compositional.lean
@@ -32,13 +32,66 @@ lemma ℱ_ℰ (d : ℰ (ƛ n) γ v) : ℱ (ℰ n) γ v := by
   | conj _ _ ih ih' => exact ⟨ih hx, ih' hx⟩
   | sub _ lt ih => exact sub_ℱ (ih hx) lt
 
-theorem lam_inversion (d : γ ⊢ ƛ n ⇓ v ⇾ v') : (γ`‚ v) ⊢ n ⇓ v' := ℱ_ℰ d
+theorem lam_inv (d : γ ⊢ ƛ n ⇓ v ⇾ v') : (γ`‚ v) ⊢ n ⇓ v' := ℱ_ℰ d
 
 lemma ℰ_lam (d : ℱ (ℰ n) γ v) : ℰ (ƛ n) γ v := match v with
 | .bot => .bot
 | .fn _ _ => .fn d
 | .conj _ _ => (ℰ_lam d.1).conj (ℰ_lam d.2)
 
-theorem lam_equiv : ℰ (ƛ n) = ℱ (ℰ n) := by ext γ v; exact ⟨ℱ_ℰ, ℰ_lam⟩
+theorem lam_equiv : ℰ (ƛ n) = ℱ (ℰ n) := by ext; exact ⟨ℱ_ℰ, ℰ_lam⟩
 
 -- https://plfa.github.io/Compositional/#equation-for-function-application
+abbrev 𝒜 (d d' : Denot Γ) : Denot Γ | γ, w => (w ⊑ ⊥) ∨ (∃ v, d γ (v ⇾ w) ∧ d' γ v)
+
+namespace Notation
+  scoped infixl:70 " ● " => 𝒜
+end Notation
+
+open Notation
+
+lemma 𝒜_ℰ (d : ℰ (l □ m) γ v) : (ℰ l ● ℰ m) γ v := by
+  generalize hx : l □ m = x at *
+  induction d with try injection hx
+  | bot => left; rfl
+  | ap d d' => subst_vars; right; rename_i v' _ _ _ _; exists v'
+  | sub _ lt ih => match ih hx with
+    | .inl lt' => left; exact lt.trans lt'
+    | .inr ⟨v', efv', ev'⟩ => right; refine ⟨v', efv'.sub ?_, ev'⟩; exact .fn .refl lt
+  | conj _ _ ih ih' => match ih hx, ih' hx with
+    | .inl lt, .inl lt' => left; exact lt.conjL lt'
+    | .inl lt, .inr ⟨v', efv', ev'⟩ =>
+        right; refine ⟨v', efv'.sub ?_, ev'⟩; refine .fn .refl ?_
+        refine .conjL ?_ .refl; exact sub_of_sub_bot lt
+    | .inr ⟨v', efv', ev'⟩, .inl lt =>
+        right; refine ⟨v', efv'.sub ?_, ev'⟩; refine .fn .refl ?_
+        refine .conjL .refl ?_; exact sub_of_sub_bot lt
+    | .inr ⟨v', efv', ev'⟩, .inr ⟨v'', efv'', ev''⟩ =>
+        right; refine ⟨v' ⊔ v'', ?_, ev'.conj ev''⟩
+        exact (efv'.conj efv'').sub fn_conj_sub_conj_fn
+
+lemma ℰ_ap : (ℰ l ● ℰ m) γ v → ℰ (l □ m) γ v
+| .inl lt => .sub .bot lt
+| .inr ⟨_, efv, ev⟩ => efv.ap ev
+
+theorem ap_equiv : ℰ (l □ m) = (ℰ l ● ℰ m) := by ext; exact ⟨𝒜_ℰ, ℰ_ap⟩
+
+abbrev 𝒱 (i : Γ ∋ ✶) (γ : Env Γ) (v : Value) : Prop := v ⊑ γ i
+
+theorem var_inv (d : ℰ (` i) γ v) : 𝒱 i γ v := by
+  generalize hx : (` i) = x at *
+  induction d with try injection hx
+  | var => subst_vars; rfl
+  | bot => exact .bot
+  | conj _ _ ih ih' => exact (ih hx).conjL (ih' hx)
+  | sub _ lt ih => exact lt.trans (ih hx)
+
+theorem var_equiv : ℰ (` i) = 𝒱 i := by ext; exact ⟨var_inv, .sub .var⟩
+
+-- https://plfa.github.io/Compositional/#congruence
+
+-- Congruence Lemmas
+
+-- Nothing to do!
+-- Since we chose to use `=` instead of `≃` in `Denotational`,
+-- everything is handled automagically!
